WIP, working on compiler proof

src/Bedrock/End2End/X25519/MontgomeryLadder.v
@@ -53,3 +53,174 @@ Definition compiler_test_out := Eval vm_compute in
 Compute
   match compiler_test_out with
   Success ((x, z), y) => Success (length x, z) | Failure e => Failure e end.
+
+Derive montladder_compiler_result SuchThat
+       (compile
+         (compile_ext_call (funname_env:=SortedListString.map))
+         (map.of_list funcs) = Some montladder_compiler_result)
+       As montladder_compiler_result_ok.
+Proof.
+  vm_compute. apply f_equal. subst; exact eq_refl.
+Qed.
+
+Check montladder_correct.
+
+Check compiler_correct.
+
+Local Arguments map.rep: clear implicits.
+Check montladder_compiler_result.
+
+Let montladder_insns := fst (fst montladder_compiler_result).
+Let montladder_finfo := snd (fst montladder_compiler_result).
+Let montladder_stack_size := snd montladder_compiler_result.
+
+Let fname := fst montladder.
+Let argnames := fst (fst (snd montladder)).
+Let retnames := snd (fst (snd montladder)).
+Let fbody := snd (snd montladder).
+Definition f_rel_pos : Z.
+  let x := constr:(map.get montladder_finfo fname) in
+  let y := eval vm_compute in x in
+  match y with
+  | Some (_, ?pos) => exact pos
+  end.
+Defined.
+
+Require Import coqutil.Map.SortedListWord.
+
+Require Import bedrock2.Map.Separation.
+Require Import coqutil.Word.Bitwidth32.
+Require Import Crypto.Arithmetic.Core.
+Require Import Crypto.Bedrock.Field.Interface.Compilation2.
+
+Local Instance mem : map.map (word.rep (width:=32)) Init.Byte.byte := SortedListWord.map _ _.
+Local Existing Instance BW32.
+
+
+(* scalars are 253 bits = 8 words *)
+Definition scalar_size_in_words := 8%nat.
+
+(* A scalar is represented as a (saturated, little-endian) array of words *)
+Definition eval_scalar_words (ws : list word.rep) : Z :=
+  Positional.eval (ModOps.weight 32 1) scalar_size_in_words
+                  (List.map (word.unsigned (word:=BasicC32Semantics.word)) ws).
+
+
+Local Instance scalar_representation : ScalarRepresentation :=
+  {| scalar := list word.rep;
+     sceval := fun ws =>  F.of_Z _ (eval_scalar_words ws);
+     Scalar := Bignum.Bignum scalar_size_in_words;
+  |}.
+
+
+Print spec_of_montladder.
+Check (
+  compiler_correct compile_ext_call compile_ext_call_correct _ (map.of_list funcs)
+                   montladder_insns montladder_finfo montladder_stack_size
+                   fname argnames retnames fbody 
+).
+
+
+Definition foo := fun post =>
+         (forall (pOUT pK pU : word.rep)
+                 (K : scalar) (U : F Field.M_pos)
+                 (out_bound : option Field.bounds) (OUT : F Field.M_pos)
+                 (R : map.rep _ _ mem -> Prop) 
+                 (tr : Semantics.trace)
+                 (mem0 : map.rep _ _ mem),
+           (FElem (field_parameters:=field_parameters)
+                  (field_representaton:=field_representation n s c)
+                  (BW:=BW32)
+                  out_bound pOUT OUT
+            ⋆ Scalar (scalar_field_parameters:=scalar_field_parameters)
+                     (ScalarRepresentation:=scalar_representation)
+                     (BW:=BW32)
+                     pK K
+            ⋆ FElem (field_parameters:=field_parameters)
+                    (field_representaton:=field_representation n s c)
+                    (BW:=BW32)
+                   (Some Field.tight_bounds) pU U ⋆ R)%sep mem0 ->
+           WeakestPrecondition.call funcs fname tr mem0 
+             [pOUT; pK; pU] post).
+
+
+Print spec_of_montladder.
+
+
+(* Postcondition extracted from spec_of_montladder *)
+Definition montladder_post (pOUT pK pU : word.rep (word:=BasicC32Semantics.word))
+          (K : scalar (scalar_field_parameters:=scalar_field_parameters)) 
+          (U : F (Field.M_pos (FieldParameters:=field_parameters)))
+          (out_bound : option (Field.bounds (BW:=BW32) (word:=BasicC32Semantics.word)
+                                            (mem:=mem)
+                                            (field_parameters:=field_parameters)
+                                            (FieldRepresentation:=field_representation n s c)))
+          (OUT : F (Field.M_pos (FieldParameters:=field_parameters)))
+          (R : map.rep word.rep Init.Byte.byte mem -> Prop)
+          (tr : Semantics.trace) : 
+  Semantics.trace -> map.rep _ _ mem -> list (word.rep (word:=BasicC32Semantics.word)) -> Prop :=
+   (fun (tr' : Semantics.trace)
+        (mem' : map.rep word.rep Init.Byte.byte mem)
+        (rets : list word.rep) =>
+      rets = [] /\
+      tr' = tr /\
+      (FElem
+         (BW:=BW32)
+         (field_representaton:=field_representation n s c)
+         (Some Field.tight_bounds) pOUT
+         (montladder_gallina scalarbits
+            (fun i : nat => Z.testbit (F.to_Z (sceval K)) (Z.of_nat i))
+            U)
+         ⋆ Scalar pK K
+         ⋆ FElem (BW:=BW32)
+                 (field_representaton:=field_representation n s c)
+                 (Some Field.tight_bounds) pU U ⋆ R)%sep
+        mem').
+
+
+(* TODO: next, plug in specific pOUT, pK, etc for argvals and add their preconditions from spec_of_montladder *)
+Lemma montladder_compiles_correctly :
+  forall (t : Semantics.trace)
+         (mH : map.rep word.rep Init.Byte.byte mem)
+         (argvals : list word.rep)
+         (initial : MetricRiscvMachine)
+         (stack_lo stack_hi ret_addr p_funcs : word.rep)
+         (Rdata Rexec : map.rep word.rep Init.Byte.byte mem -> Prop),
+         montladder_stack_size <=
+         word.unsigned (word.sub stack_hi stack_lo) /
+         SeparationLogic.bytes_per_word ->
+         word.unsigned (word.sub stack_hi stack_lo)
+         mod SeparationLogic.bytes_per_word = 0 ->
+         getPc (getMachine initial) = word.add p_funcs (word.of_Z f_rel_pos) ->
+         map.get (getRegs (getMachine initial)) RegisterNames.ra =
+         Some ret_addr ->
+         word.unsigned ret_addr mod 4 = 0 ->
+         map.getmany_of_list (getRegs (getMachine initial))
+           (firstn (Datatypes.length argnames) (reg_class.all reg_class.arg)) =
+         Some argvals ->
+         getLog (getMachine initial) = t ->
+         LowerPipeline.machine_ok p_funcs stack_lo stack_hi montladder_insns
+           mH Rdata Rexec initial ->
+         FlatToRiscvCommon.runsTo initial
+           (fun final : MetricRiscvMachine =>
+            exists
+              (mH' : map.rep word.rep Init.Byte.byte mem) 
+            (retvals : list word.rep),
+              map.getmany_of_list (getRegs (getMachine final))
+                (firstn (Datatypes.length retnames)
+                   (reg_class.all reg_class.arg)) = 
+              Some retvals /\
+              ?post (getLog (getMachine final)) mH' retvals /\
+              map.agree_on LowerPipeline.callee_saved
+                (getRegs (getMachine initial)) (getRegs (getMachine final)) /\
+              getPc (getMachine final) = ret_addr /\
+              LowerPipeline.machine_ok p_funcs stack_lo stack_hi
+                montladder_insns mH' Rdata Rexec final).
+
+
+Check (
+  compiler_correct compile_ext_call compile_ext_call_correct _ (map.of_list funcs)
+                   montladder_insns montladder_finfo montladder_stack_size
+                   fname argnames retnames fbody _ _ _ _ _ _ _
+     _
+).
